Stabilisation.thy
@@ -1,0 +1,363 @@
+theory Stabilisation
+  imports SepLogic
+begin
+
+section \<open>Helper Lemmas\<close>
+
+lemma le_map_le_iff_sepadd:
+  \<open>(a \<subseteq>\<^sub>m b) = (\<exists>c. dom a \<inter> dom c = {} \<and> b = a ++ c)\<close>
+  by (metis dom_restrict inf_compl_bot_right map_add_comm map_le_map_add map_le_split)
+
+lemma disjoint_dom_map_add_restrict_distrib:
+  \<open>dom a \<inter> dom b = {} \<Longrightarrow> (a ++ b) |` A = a |` A ++ b |` A\<close>
+  by (simp add: fun_eq_iff restrict_map_def map_add_def)
+
+lemma antidom_restrict_eq[simp]:
+  \<open>a |` (- dom a) = Map.empty\<close>
+  by (force simp add: restrict_map_def subset_iff domIff)
+
+lemma dom_subset_restrict_eq:
+  \<open>dom a \<subseteq> A \<Longrightarrow>  a |` A = a\<close>
+  by (force simp add: restrict_map_def subset_iff domIff)
+
+lemmas dom_disjoint_restrict_eq =
+  dom_subset_restrict_eq[OF iffD1[OF disjoint_eq_subset_Compl]]
+
+lemma transp_subrel_compp_smaller:
+  \<open>transp S \<Longrightarrow> R \<le> S \<Longrightarrow> S OO R \<le> S\<close>
+  \<open>transp S \<Longrightarrow> R \<le> S \<Longrightarrow> R OO S \<le> S\<close>
+  by (meson order.refl order.trans relcompp_mono transp_relcompp_less_eq)+
+
+lemma rel_le_rtranscp_relcompp_absorb:
+  \<open>R \<le> S \<Longrightarrow> S\<^sup>*\<^sup>* OO R\<^sup>*\<^sup>* = S\<^sup>*\<^sup>*\<close>
+  \<open>R \<le> S \<Longrightarrow> R\<^sup>*\<^sup>* OO S\<^sup>*\<^sup>* = S\<^sup>*\<^sup>*\<close>
+   apply -
+   apply (rule antisym)
+    apply (metis rtranclp_mono transp_rtranclp transp_subrel_compp_smaller(1))
+   apply force
+  apply (rule antisym)
+   apply (simp add: rtranclp_mono transp_subrel_compp_smaller(2))
+  apply force
+  done
+
+section \<open>Finite Heaps\<close>
+
+typedef ('p,'v) heap = \<open>{h::'p \<rightharpoonup> 'v. finite (dom h)}\<close>
+  by (rule exI[where x=Map.empty], force)
+
+setup_lifting type_definition_heap
+
+lemma eq_Rep_heap_iff:
+  \<open>a = Rep_heap a' \<longleftrightarrow> a' = Abs_heap a \<and> finite (dom a)\<close>
+  \<open>Rep_heap a' = a \<longleftrightarrow> a' = Abs_heap a \<and> finite (dom a)\<close>
+  by (metis Abs_heap_inverse Rep_heap Rep_heap_inverse mem_Collect_eq)+
+
+lemma eq_Abs_heap_iff:
+  \<open>finite (dom a) \<Longrightarrow> a' = Abs_heap a \<longleftrightarrow> a = Rep_heap a'\<close>
+  \<open>finite (dom a) \<Longrightarrow> Abs_heap a = a' \<longleftrightarrow> a = Rep_heap a'\<close>
+  by (force simp add: eq_Rep_heap_iff)+
+
+lemma finite_dom_Rep_heap[simp]:
+  \<open>finite (dom (Rep_heap a))\<close>
+  using eq_Rep_heap_iff by auto
+
+
+instantiation heap :: (type,type) cancel_seplogic
+begin
+
+lift_definition disjoint_heap :: \<open>('a,'b) heap \<Rightarrow> ('a,'b) heap \<Rightarrow> bool\<close> is
+  \<open>\<lambda>a b. dom a \<inter> dom b = {}\<close> .
+
+lift_definition plus_heap :: \<open>('a,'b) heap \<Rightarrow> ('a,'b) heap \<Rightarrow> ('a,'b) heap\<close> is \<open>(++)\<close>
+  by simp
+
+lift_definition zero_heap :: \<open>('a,'b) heap\<close> is \<open>Map.empty\<close>
+  by simp
+
+lift_definition bot_heap :: \<open>('a,'b) heap\<close> is \<open>Map.empty\<close>
+  by simp
+
+lift_definition less_eq_heap :: \<open>('a,'b) heap \<Rightarrow> ('a,'b) heap \<Rightarrow> bool\<close> is
+  \<open>(\<subseteq>\<^sub>m)\<close> .
+
+definition less_heap :: \<open>('a,'b) heap \<Rightarrow> ('a,'b) heap \<Rightarrow> bool\<close> where
+  \<open>less_heap a b \<equiv> a \<le> b \<and> \<not>(b \<le> a)\<close>
+
+lift_definition minus_heap :: \<open>('a,'b) heap \<Rightarrow> ('a,'b) heap \<Rightarrow> ('a,'b) heap\<close> is
+  \<open>\<lambda>a b. a |` (- dom b)\<close> by simp
+
+
+instance
+  apply standard
+                  apply (simp add: less_heap_def; fail)
+                 apply (simp add: less_eq_heap_def; fail)
+                apply (force intro: map_le_trans simp add: less_eq_heap_def)
+               apply (force dest: map_le_antisym simp add: less_eq_heap_def Rep_heap_inject)
+              apply (simp add: less_eq_heap_def bot_heap_def Abs_heap_inverse; fail)
+             apply (force simp add: disjoint_heap_def)
+            apply (simp add: disjoint_heap_def zero_heap_def eq_Abs_heap_iff; fail)
+           apply (simp add: disjoint_heap_def plus_heap_def Abs_heap_inverse
+      Int_Un_distrib sup_commute; fail)
+          apply (simp add: disjoint_heap_def plus_heap_def less_eq_heap_def eq_Abs_heap_iff
+      le_map_le_iff_sepadd, metis dom_map_add eq_Rep_heap_iff finite_Un; fail)
+         apply (simp add: disjoint_heap_def plus_heap_def Abs_heap_inverse; fail)
+        apply (fastforce dest: map_add_comm simp add: disjoint_heap_def plus_heap_def)
+           apply (simp add: plus_heap_def zero_heap_def Abs_heap_inverse Rep_heap_inverse; fail)
+      apply (simp add: plus_heap_def minus_heap_def disjoint_heap_def
+      Abs_heap_inverse Rep_heap_inverse
+      disjoint_dom_map_add_restrict_distrib Int_commute dom_disjoint_restrict_eq; fail)
+     apply (simp add: plus_heap_def minus_heap_def disjoint_heap_def
+      Abs_heap_inverse Int_commute; fail)
+    apply (simp add: plus_heap_def minus_heap_def disjoint_heap_def Abs_heap_inverse; fail)
+
+   apply (simp add: plus_heap_def minus_heap_def disjoint_heap_def
+      Abs_heap_inverse eq_Abs_heap_iff map_restrict_un_eq)
+   apply (metis dom_subset_restrict_eq inf_sup_ord(2) map_restrict_un_eq sup_commute sup_neg_inf)
+
+  apply (simp add: minus_heap_def plus_heap_def disjoint_heap_def eq_Abs_heap_iff Abs_heap_inverse,
+      metis Compl_Int dom_disjoint_restrict_eq inf_bot_right map_restrict_un_eq; fail)
+  done
+
+end
+
+
+lift_definition dom_heap :: \<open>('a,'b) heap \<Rightarrow> 'a set\<close> is \<open>dom\<close> .
+
+lift_definition restrict_heap :: \<open>('a,'b) heap \<Rightarrow> 'a set \<Rightarrow> ('a,'b) heap\<close>
+  (infixl \<open>|`\<^sub>h\<close> 110) is \<open>(|`)\<close>
+  by simp
+
+lemma restrict_heap_un_eq: \<open>h |`\<^sub>h (A \<union> B) = h |`\<^sub>h A + h |`\<^sub>h B\<close>
+  by (simp add: restrict_heap_def plus_heap_def Abs_heap_inverse map_restrict_un_eq)
+
+lemma restrict_heap_add_eq[simp]:
+  \<open>(a + b) |`\<^sub>h A = a |`\<^sub>h A + b |`\<^sub>h A\<close>
+  by (simp add: disjoint_heap_def restrict_heap_def plus_heap_def Abs_heap_inverse
+      Abs_heap_inject, simp add: map_add_def restrict_map_def fun_eq_iff)
+
+lemma dom_restrict_heap_eq[simp]: \<open>dom_heap (h |`\<^sub>h A) = dom_heap h \<inter> A\<close>
+  by (simp add: dom_heap.rep_eq restrict_heap.rep_eq)
+
+lemma dom_plus_heap_eq[simp]: \<open>dom_heap (h1 + h2) = dom_heap h1 \<union> dom_heap h2\<close>
+  by (simp add: dom_heap.rep_eq plus_heap.rep_eq sup_commute)
+
+lemma restrict_heap_ge_dom_eq[simp]: \<open>dom_heap h \<subseteq> A \<Longrightarrow> h |`\<^sub>h A = h\<close>
+  by (simp add: dom_heap.rep_eq restrict_heap_def eq_Abs_heap_iff,
+      metis inf.absorb_iff1 map_le_refl map_le_restrict_eq restrict_restrict)
+
+lemma restrict_disjoint_dom[simp]: \<open>a ## b \<Longrightarrow> a |`\<^sub>h dom_heap b = 0\<close>
+  by (simp add: dom_heap_def restrict_heap_def disjoint_heap_def zero_heap_def Abs_heap_inject,
+      force simp add: restrict_map_def fun_eq_iff domIff)
+
+
+section \<open>Stabilisation\<close>
+
+definition swstable_pred
+  :: \<open>('a \<Rightarrow> bool) \<Rightarrow> ('a \<Rightarrow> 'a \<Rightarrow> bool) \<Rightarrow> ('a \<Rightarrow> bool)\<close>
+  ("\<lfloor> _ \<rfloor>\<^bsub>_\<^esub>" [0,0] 90)
+  where
+  \<open>\<lfloor> P \<rfloor>\<^bsub>R\<^esub> \<equiv> \<lambda>s. \<forall>s'. R\<^sup>*\<^sup>* s s' \<longrightarrow> P s'\<close>
+
+definition wsstable_pred
+  :: \<open>('a \<Rightarrow> bool) \<Rightarrow> ('a \<Rightarrow> 'a \<Rightarrow> bool) \<Rightarrow> ('a \<Rightarrow> bool)\<close>
+  ("\<lceil> _ \<rceil>\<^bsub>_\<^esub>" [0,0] 90)
+  where
+  \<open>\<lceil> P \<rceil>\<^bsub>R\<^esub> \<equiv> \<lambda>s'. \<exists>s. R\<^sup>*\<^sup>* s s' \<and> P s\<close>
+
+subsection \<open>basic logical properties\<close>
+
+lemma swstable_weaker: \<open>\<lfloor> P \<rfloor>\<^bsub>R\<^esub> \<le> P\<close>
+  by (force simp add: swstable_pred_def)
+
+lemma wsstable_stronger: \<open>P \<le> \<lceil> P \<rceil>\<^bsub>R\<^esub>\<close>
+  by (force simp add: wsstable_pred_def)
+
+subsection \<open>(semi)distributivity properties\<close>
+
+lemma swstable_conj_distrib: \<open>\<lfloor> P \<sqinter> Q \<rfloor>\<^bsub>R\<^esub> = \<lfloor> P \<rfloor>\<^bsub>R\<^esub> \<sqinter> \<lfloor> Q \<rfloor>\<^bsub>R\<^esub>\<close>
+  by (force simp add: swstable_pred_def)
+
+lemma swstable_disj_semidistrib: \<open>\<lfloor> P \<rfloor>\<^bsub>R\<^esub> \<squnion> \<lfloor> Q \<rfloor>\<^bsub>R\<^esub> \<le> \<lfloor> P \<squnion> Q \<rfloor>\<^bsub>R\<^esub>\<close>
+  by (force simp add: swstable_pred_def)
+
+lemma wsstable_disj_distrib: \<open>\<lceil> P \<squnion> Q \<rceil>\<^bsub>R\<^esub> = \<lceil> P \<rceil>\<^bsub>R\<^esub> \<squnion> \<lceil> Q \<rceil>\<^bsub>R\<^esub>\<close>
+  by (force simp add: wsstable_pred_def)
+
+lemma wsstable_conj_semidistrib: \<open>\<lceil> P \<sqinter> Q \<rceil>\<^bsub>R\<^esub> \<le> \<lceil> P \<rceil>\<^bsub>R\<^esub> \<sqinter> \<lceil> Q \<rceil>\<^bsub>R\<^esub>\<close>
+  by (force simp add: wsstable_pred_def)
+
+subsection \<open>Rely Monotonicity\<close>
+
+lemma swstable_rely_antimono: \<open>R \<le> S \<Longrightarrow> \<lfloor> P \<rfloor>\<^bsub>S\<^esub> \<le> \<lfloor> P \<rfloor>\<^bsub>R\<^esub>\<close>
+  using mono_rtranclp
+  by (force simp add: swstable_pred_def le_fun_def)
+
+lemma wsstable_rely_mono: \<open>R \<le> S \<Longrightarrow> \<lceil> P \<rceil>\<^bsub>R\<^esub> \<le> \<lceil> P \<rceil>\<^bsub>S\<^esub>\<close>
+  using mono_rtranclp
+  by (force simp add: wsstable_pred_def le_fun_def)
+
+subsection \<open>nested stabilisation\<close>
+
+lemma wsstable_absorb[simp]:
+  assumes \<open>R\<^sup>*\<^sup>* = Ra\<^sup>*\<^sup>* OO Rb\<^sup>*\<^sup>*\<close>
+  shows \<open>\<lceil> \<lceil> P \<rceil>\<^bsub>Ra\<^esub> \<rceil>\<^bsub>Rb\<^esub> = \<lceil> P \<rceil>\<^bsub>R\<^esub>\<close>
+  by (force simp add: assms wsstable_pred_def relcompp_apply fun_eq_iff)
+
+lemma wsstable_absorb1[simp]: \<open>R \<le> R' \<Longrightarrow> \<lceil> \<lceil> P \<rceil>\<^bsub>R\<^esub> \<rceil>\<^bsub>R'\<^esub> = \<lceil> P \<rceil>\<^bsub>R'\<^esub>\<close>
+  by (simp add: rel_le_rtranscp_relcompp_absorb)
+
+lemma wsstable_absorb2[simp]: \<open>R \<le> R' \<Longrightarrow> \<lceil> \<lceil> P \<rceil>\<^bsub>R'\<^esub> \<rceil>\<^bsub>R\<^esub> = \<lceil> P \<rceil>\<^bsub>R'\<^esub>\<close>
+  by (simp add: rel_le_rtranscp_relcompp_absorb)
+
+lemma swstable_absorb[simp]:
+  \<open>R\<^sup>*\<^sup>* = Rb\<^sup>*\<^sup>* OO Ra\<^sup>*\<^sup>* \<Longrightarrow> \<lfloor> \<lfloor> P \<rfloor>\<^bsub>Ra\<^esub> \<rfloor>\<^bsub>Rb\<^esub> = \<lfloor> P \<rfloor>\<^bsub>R\<^esub>\<close>
+  by (force simp add: swstable_pred_def relcompp_apply imp_ex imp_conjL fun_eq_iff)
+
+lemma swstable_absorb1[simp]: \<open>R \<le> R' \<Longrightarrow> \<lfloor> \<lfloor> P \<rfloor>\<^bsub>R\<^esub> \<rfloor>\<^bsub>R'\<^esub> = \<lfloor> P \<rfloor>\<^bsub>R'\<^esub>\<close>
+  by (simp add: rel_le_rtranscp_relcompp_absorb)
+
+lemma swstable_absorb2[simp]: \<open>R \<le> R' \<Longrightarrow> \<lfloor> \<lfloor> P \<rfloor>\<^bsub>R'\<^esub> \<rfloor>\<^bsub>R\<^esub> = \<lfloor> P \<rfloor>\<^bsub>R'\<^esub>\<close>
+  by (simp add: rel_le_rtranscp_relcompp_absorb)
+
+
+lemma wsstable_swstable_absorb[simp]: \<open>R \<le> R' \<Longrightarrow> \<lceil> \<lfloor> P \<rfloor>\<^bsub>R'\<^esub> \<rceil>\<^bsub>R\<^esub> = \<lfloor> P \<rfloor>\<^bsub>R'\<^esub>\<close>
+  unfolding wsstable_pred_def swstable_pred_def
+  by (metis (opaque_lifting) predicate2D rtranclp.rtrancl_refl rtranclp_trans rtranclp_mono)
+
+lemma swstable_wsstable_absorb[simp]: \<open>R \<le> R' \<Longrightarrow> \<lfloor> \<lceil> P \<rceil>\<^bsub>R'\<^esub> \<rfloor>\<^bsub>R\<^esub> = \<lceil> P \<rceil>\<^bsub>R'\<^esub>\<close>
+  unfolding wsstable_pred_def swstable_pred_def
+  by (metis (opaque_lifting) predicate2D rtranclp.rtrancl_refl rtranclp_trans rtranclp_mono)
+
+
+context seplogic
+begin
+
+(*
+
+(* should this be true? *)
+lemma sepdomeq_substates_equal:
+  \<open>\<And>a a1 a2. a1 \<le> a \<Longrightarrow> a2 \<le> a \<Longrightarrow> sepdomeq a1 a2 \<Longrightarrow> a1 = a2\<close>
+  oops                                                                
+
+assumes rely_substate_result_consistent:
+  \<open>\<And>a b b'. R\<^sup>*\<^sup>* a b \<Longrightarrow> R\<^sup>*\<^sup>* a b' \<Longrightarrow> b' \<le> b \<Longrightarrow> b' = b\<close>
+
+lemma
+  assumes rely_same_dom: \<open>\<And>a b. R\<^sup>*\<^sup>* a b \<Longrightarrow> sepdomeq a b\<close>
+  assumes rely_additivity_of_update:
+    \<open>\<And>a1 a2 b. a1 ## a2 \<Longrightarrow> R\<^sup>*\<^sup>* (a1 + a2) b \<Longrightarrow> \<exists>b1 b2. R\<^sup>*\<^sup>* a1 b1 \<and> R\<^sup>*\<^sup>* a2 b2 \<and> b = b1 + b2 \<and> b1 ## b2\<close>
+  shows
+    \<open>\<And>a b a' b'. R\<^sup>*\<^sup>* a b \<Longrightarrow> a' \<le> a \<Longrightarrow> \<exists>b'\<le> b. R\<^sup>*\<^sup>* a' b' \<and> sepdomeq a' b'\<close>
+  by (simp add: le_iff_sepadd, blast dest: rely_additivity_of_update intro: rely_same_dom)
+*)
+
+lemma swstable_sepconj_semidistrib:
+  fixes P Q :: \<open>'a \<Rightarrow> bool\<close>
+  assumes rely_additivity_of_update:
+    \<open>\<And>a1 a2 b. a1 ## a2 \<Longrightarrow> R\<^sup>*\<^sup>* (a1 + a2) b \<Longrightarrow> \<exists>b1 b2. b1 ## b2 \<and> b = b1 + b2 \<and> R\<^sup>*\<^sup>* a1 b1 \<and> R\<^sup>*\<^sup>* a2 b2\<close>
+  shows \<open>(\<lfloor> P \<rfloor>\<^bsub>R\<^esub> \<^emph> \<lfloor> Q \<rfloor>\<^bsub>R\<^esub>) s \<Longrightarrow> (\<lfloor> P \<^emph> Q \<rfloor>\<^bsub>R\<^esub>) s\<close>
+  using rely_additivity_of_update
+  by (simp add: swstable_pred_def sepconj_def le_fun_def, metis)
+
+lemma wsstable_sepconj_semidistrib:
+  fixes P Q :: \<open>'a \<Rightarrow> bool\<close>
+  assumes rely_additivity_of_update:
+    \<open>\<And>a1 a2 b. a1 ## a2 \<Longrightarrow> R\<^sup>*\<^sup>* (a1 + a2) b \<Longrightarrow> \<exists>b1 b2. b1 ## b2 \<and> b = b1 + b2 \<and> R\<^sup>*\<^sup>* a1 b1 \<and> R\<^sup>*\<^sup>* a2 b2\<close>
+  assumes rely_same_dom: \<open>\<And>a b. R\<^sup>*\<^sup>* a b \<Longrightarrow> sepdomeq a b\<close>
+  shows \<open>\<lceil> P \<^emph> Q \<rceil>\<^bsub>R\<^esub> \<le> \<lceil> P \<rceil>\<^bsub>R\<^esub> \<^emph> \<lceil> Q \<rceil>\<^bsub>R\<^esub>\<close>
+  using rely_additivity_of_update
+  by (simp add: wsstable_pred_def sepconj_def le_fun_def, metis)
+
+end
+
+
+section \<open>Seplogic stabilisation\<close>
+
+lemma swstable_sepconj_semidistrib:
+  fixes P Q :: \<open>('a,'b) heap \<Rightarrow> bool\<close>
+  assumes rely_restrict_consistent: \<open>\<And>a b A. R\<^sup>*\<^sup>* a b \<Longrightarrow> R\<^sup>*\<^sup>* (a |`\<^sub>h A) (b |`\<^sub>h A)\<close>
+  assumes rely_same_dom: \<open>\<And>a b. R\<^sup>*\<^sup>* a b \<Longrightarrow> dom_heap a = dom_heap b\<close>
+  shows \<open>\<lfloor> P \<rfloor>\<^bsub>R\<^esub> \<^emph> \<lfloor> Q \<rfloor>\<^bsub>R\<^esub> \<le> \<lfloor> P \<^emph> Q \<rfloor>\<^bsub>R\<^esub>\<close>
+proof -
+  have rely_additivity:
+    \<open>\<And>a1 a2 b. a1 ## a2 \<Longrightarrow> R\<^sup>*\<^sup>* (a1 + a2) b \<Longrightarrow> \<exists>b1 b2. R\<^sup>*\<^sup>* a1 b1 \<and> R\<^sup>*\<^sup>* a2 b2 \<and> b = b1 + b2 \<and> b1 ## b2\<close>
+    apply (frule rely_same_dom)
+    apply (rule_tac x=\<open>b |`\<^sub>h dom_heap a1\<close> in exI)
+    apply (rule_tac x=\<open>b |`\<^sub>h dom_heap a2\<close> in exI)
+    apply (intro conjI)
+       apply (drule_tac A=\<open>dom_heap a1\<close> in rely_restrict_consistent, simp add: disjoint_symm; fail)
+      apply (drule_tac A=\<open>dom_heap a2\<close> in rely_restrict_consistent, simp add: disjoint_symm; fail)
+     apply (simp add: restrict_heap_def plus_heap_def dom_heap_def Abs_heap_inverse eq_Abs_heap_iff
+        map_restrict_un_eq[symmetric] dom_subset_restrict_eq sup_commute; fail)
+    apply (force simp add: restrict_heap_def  dom_heap_def disjoint_heap_def Abs_heap_inverse)
+    done
+  then show ?thesis
+    by (metis predicate1I swstable_sepconj_semidistrib)
+qed
+
+lemma wsstable_sepconj_semidistrib:
+  fixes P Q :: \<open>('a,'b) heap \<Rightarrow> bool\<close>
+  assumes rely_restrict_consistent: \<open>\<And>a b A. R\<^sup>*\<^sup>* a b \<Longrightarrow> R\<^sup>*\<^sup>* (a |`\<^sub>h A) (b |`\<^sub>h A)\<close>
+  assumes rely_same_dom: \<open>\<And>a b. R\<^sup>*\<^sup>* a b \<Longrightarrow> dom_heap a = dom_heap b\<close>
+  shows \<open>\<lceil> P \<^emph> Q \<rceil>\<^bsub>R\<^esub> \<le> \<lceil> P \<rceil>\<^bsub>R\<^esub> \<^emph> \<lceil> Q \<rceil>\<^bsub>R\<^esub>\<close>
+  apply (clarsimp simp add: wsstable_pred_def sepconj_def le_fun_def)
+  apply (rename_tac s' h1 h2)
+  apply (rule_tac x=\<open>s' |`\<^sub>h dom_heap h1\<close> in exI)
+  apply (rule_tac x=\<open>s' |`\<^sub>h dom_heap h2\<close> in exI)
+  apply (frule rely_same_dom)
+  apply (frule_tac A=\<open>dom_heap h1\<close> in rely_restrict_consistent)
+  apply (frule_tac A=\<open>dom_heap h2\<close> in rely_restrict_consistent)
+  apply (simp add: restrict_heap_def disjoint_heap_def dom_heap_def plus_heap_def
+      Abs_heap_inverse eq_Abs_heap_iff)
+  apply (intro conjI)
+     apply blast
+    apply (metis dom_subset_restrict_eq dual_order.refl map_restrict_un_eq sup_commute)
+   apply (metis Rep_heap_inverse map_add_comm map_le_iff_map_add_commute map_le_restrict_eq)
+  apply (metis Rep_heap_inverse map_le_map_add map_le_restrict_eq)
+  done
+
+context cancel_seplogic
+begin
+
+lemma swstable_sepconj_semidistrib:
+  fixes P Q :: \<open>'a \<Rightarrow> bool\<close>
+  assumes rely_restrict_consistent: \<open>\<And>a b c. R\<^sup>*\<^sup>* a b \<Longrightarrow> R\<^sup>*\<^sup>* (a - c) (b - c)\<close>
+  assumes rely_same_dom: \<open>\<And>a b. R\<^sup>*\<^sup>* a b \<Longrightarrow> sepdomeq a b\<close>
+  shows \<open>\<lfloor> P \<rfloor>\<^bsub>R\<^esub> \<^emph> \<lfloor> Q \<rfloor>\<^bsub>R\<^esub> \<le> \<lfloor> P \<^emph> Q \<rfloor>\<^bsub>R\<^esub>\<close>
+  apply (clarsimp simp add: swstable_pred_def sepconj_def le_fun_def)
+  apply (rule_tac x=\<open>s' - h2\<close> in exI)
+  apply (rule_tac x=\<open>s' - h1\<close> in exI)
+  apply (frule_tac c=h1 in rely_restrict_consistent)
+  apply (frule_tac c=h2 in rely_restrict_consistent)
+  apply (intro conjI)
+     apply (force dest: rely_same_dom rely_restrict_consistent simp add: disjoint_symm sepdomeq_def)
+    defer
+    apply force
+   apply force
+  apply (drule rely_same_dom)+
+  apply (simp add: disjoint_symm partial_add_commute state_minus_generic_split[symmetric])
+  done
+
+lemma wsstable_sepconj_semidistrib:
+  fixes P Q :: \<open>'a \<Rightarrow> bool\<close>
+  assumes rely_restrict_consistent: \<open>\<And>a b c. R\<^sup>*\<^sup>* a b \<Longrightarrow> R\<^sup>*\<^sup>* (a - c) (b - c)\<close>
+  assumes rely_same_dom: \<open>\<And>a b. R\<^sup>*\<^sup>* a b \<Longrightarrow> sepdomeq a b\<close>
+  shows \<open>\<lceil> P \<^emph> Q \<rceil>\<^bsub>R\<^esub> \<le> \<lceil> P \<rceil>\<^bsub>R\<^esub> \<^emph> \<lceil> Q \<rceil>\<^bsub>R\<^esub>\<close>
+  apply (clarsimp simp add: wsstable_pred_def sepconj_def le_fun_def)
+  apply (rename_tac s' h1 h2)
+  apply (rule_tac x=\<open>s' - h2\<close> in exI)
+  apply (rule_tac x=\<open>s' - h1\<close> in exI)
+  apply (frule_tac c=h1 in rely_restrict_consistent)
+  apply (frule_tac c=h2 in rely_restrict_consistent)
+  apply (intro conjI)
+     apply (force dest: rely_same_dom rely_restrict_consistent simp add: disjoint_symm sepdomeq_def)
+    defer
+    apply force
+   apply force
+  apply (drule rely_same_dom)+
+  apply (simp add: disjoint_symm partial_add_commute state_minus_generic_split[symmetric])
+  done
+
+end
+
+end
